\textbf{Linear Independence of Bernstein-Bezier Basis Functions} show that, for all $n \geq 0$, 
$$\sigma_{i = 0}^n c_i \binom{n}{i} x^i (1 - x)^{n - i} = 0 \rightarrow c_i = 0, i = 0, \cdots, n.$$

\textbf{Proof}\\
In order to show that the Bernstein Bezier functions are linearly independent, we first note that 
$$B_{k, n}(t) = \Sigma_{i = k}^n (-1)^{i - k} \binom{n}{i} \binom{i}{k}t^i$$
which is simply a change of basis to the power basis. Now, assume that the Bernstein-Bezier functions are not linearly independent. Then for some set of $c_i$, we have that
\begin{align*}
 0 &= \Sigma_{i = 0}^n B_{i, n}(t) \\
 &= c_0 \Sigma_{i = 0}^n (-1)^i \binom{n}{i} \binom{i}{0}t^i + c_1 \Sigma_{i = 1}^n (-1)^{i - 1} \binom{n}{i} \binom{i}{1}t^i + \cdots + c_n \Sigma_{i = n}^n (-1)^{i - n} \binom{n}{i} \binom{i}{n}t^i\\
 &= c_0 + \Sigma_{i = 0}^1 \binom{n}{1} \binom{1}{1}t^1+ \cdots + \Sigma_{i = 0}^n \binom{n}{n} \binom{n}{n}t^n
 \end{align*}

 Since the power basis is linearly independent, we see that in order to have a linearly dependent set, we require that 
 \begin{align*}
c_0 &= 0\\
0 &= \Sigma_{i = 0}^1 \binom{n}{1} \binom{1}{1}\\
&\vdots\\
&= \Sigma_{i = 0}^n \binom{n}{n} \binom{n}{n}
 \end{align*}
 which implies that $c_0 = c_1 = \cdots = c_n = 0$. Thus, the Bernstein Bezier functions are linearly independent.