\textbf{Recurrence Relation} Consider the inner product $$(f, g) - \int_{-1}^1 f(x) g(x) dx.$$ Use the recurrence relation from the previous problem to compute $Q_i \text{ for } i = 0, 1, 2, 3, 4, 5.$

\textbf{solution}\\
We are already given $Q_0 = 1$. We then get that
\begin{align*}
Q_1 &= x - \frac{\int_{-1}^1x dx}{\int_{-1}^1 x^2 dx} = x\\
Q_2 &= (x - \frac{\int_{-1}^1 x^3 dx}{\int_{-1}^1} x^2 dx)x - \frac{\int_{-1}^1 x^2 dx}{\int_{-1}^1 dx} = x^2 - 1/3\\
Q_3 &= x(x^2 - 1/3) - \frac{\int_{-1}^1 (x^3 - 1/3x)x dx}{\int_{-1}^1 x^2 dx} = x^3 - 1/3x - 3/15x = x^3 - 3/5x\\
Q_4 &= x(x^3 - 3/5x) - \frac{\int_{-1}^1 x(x^3 - 3/5x)(x^2 - 1/3)dx} {\int_{-1}^1 (x^2 - 1/3)^2 dx} \\ 
&= x(x^3 - 3/5x) - 9/35(x^2 - 1/3) = x^4- \frac{6}{7}x^2 - \frac{3}{35}\\
Q_5 &= x(x^4- \frac{6}{7}x^2 - \frac{3}{35}) - \frac{\int_{-1}^1 x(x^4- \frac{6}{7}x^2 - \frac{3}{35})(x^3 - 3/5x) dx}{\int_{-1}^1 (x^3 - 3/5x)^2 dx}\\
&= x^5 - \frac{10}{9}x^3 - \frac{5}{21}x
\end{align*}
Here, we have used the fact that $a_n$ over the interval $[-1, 1]$ is the integral of an odd function. Because of the symmetric interval, this integral is 0. 
